updated lock_server

Test/591tests/lock_server.dfy
@@ -15,19 +15,6 @@ predicate RelationSemaphore(m: DafnyState, s: Server)
     && m.servers[s.id].semaphore
 }
 
-// c1 should be not changing if it is != c2
-// predicate RelationLinkStable(m : DafnyState, m' : DafnyState, c1: Client, c2: Client, s: Server) {
-//     c1.id != c2.id ==> RelationLink(m, c1, s) == RelationLink(m', c1, s)  link_c1_s_next
-// }
-
-predicate RelationDifferentClients(m: DafnyState, c1: Client, c2: Client){
-    c1.id != c2.id
-}
-
-predicate RelationDifferentServers(m: DafnyState, s1: Server, s2: Server){
-    s1.id != s2.id
-}
-
 predicate RelationServerExists(m: DafnyState, s: Server){
     s in m.servers
 }
@@ -36,10 +23,20 @@ predicate RelationClientExists(m: DafnyState, c: Client){
     c in m.clients
 }
 
+predicate RelationDifferentClients(m: DafnyState, c1: Client, c2: Client){
+    && RelationClientExists(m, c1)
+    && RelationClientExists(m, c2)
+    && c1.id != c2.id
+}
+
+predicate RelationDifferentServers(m: DafnyState, s1: Server, s2: Server){
+    && RelationServerExists(m, s1)
+    && RelationServerExists(m, s2)
+    && s1.id != s2.id
+}
+
 predicate Init(m: DafnyState) {
-    // && (forall s: Server :: s in m.servers ==> RelationSemaphore(m, s))
     && (forall s: Server :: RelationServerExists(m, s) ==> RelationSemaphore(m, s))
-    // && (forall s: Server, c: Client :: s in m.servers && c in m.clients ==> !RelationLink(m, c, s))
     && (forall s: Server, c: Client :: ((RelationServerExists(m, s) && RelationClientExists(m, c)) ==> !RelationLink(m, c, s)))
 }
 
@@ -50,12 +47,9 @@ predicate ActionConnect(m: DafnyState, m': DafnyState) {
         && RelationLink(m', c, s)
         && !RelationSemaphore(m', s)
 
-        // TODO: might need to ensure client/server is in m.clients/m.servers on left side of implication
-        // && forall cf: Client, sf: Server :: (cf.id != c.id ==> RelationLink(m, cf, sf) == RelationLink(m', cf, sf))
-        // && forall cf: Client, sf: Server :: RelationLinkStable(m, cf, c, sf)
-        && forall cf: Client, sf: Server :: (RelationDifferentClients(m, cf, c) ==> RelationLink(m, cf, sf) == RelationLink(m', cf, sf))
+        && (forall cf: Client, sf: Server :: (RelationDifferentClients(m, cf, c) ==> RelationLink(m, cf, sf) == RelationLink(m', cf, sf)))
         
-        && forall sf: Server :: (RelationDifferentServers(m, sf, s) ==> RelationSemaphore(m, sf) == RelationSemaphore(m', sf))
+        && (forall sf: Server :: (RelationDifferentServers(m, sf, s) ==> RelationSemaphore(m, sf) == RelationSemaphore(m', sf)))
 }
 
 predicate ActionDisconnect(m: DafnyState, m': DafnyState) {
@@ -65,9 +59,9 @@ predicate ActionDisconnect(m: DafnyState, m': DafnyState) {
         && !RelationLink(m', c, s)
         && RelationSemaphore(m', s)
 
-        && forall cf: Client, sf: Server :: (RelationDifferentClients(m, cf, c) ==> RelationLink(m, cf, sf) == RelationLink(m', cf, sf))
+        && (forall cf: Client, sf: Server :: (RelationDifferentClients(m, cf, c) ==> RelationLink(m, cf, sf) == RelationLink(m', cf, sf)))
         
-        && forall sf: Server :: (RelationDifferentServers(m, sf, s) ==> RelationSemaphore(m, sf) == RelationSemaphore(m', sf))
+        && (forall sf: Server :: (RelationDifferentServers(m, sf, s) ==> RelationSemaphore(m, sf) == RelationSemaphore(m', sf)))
 
 }
 
@@ -77,11 +71,7 @@ predicate Next(m:DafnyState, m':DafnyState) {
 }
 
 
-lemma Invariant(m: DafnyState) 
-    ensures forall c1: Client, c2:Client, s: Server :: 
-    (RelationClientExists(m, c1) && RelationClientExists(m, c2) && RelationServerExists(m, s)) ==> (RelationLink(m, c1, s) && RelationLink(m, c2, s) ==> !RelationDifferentClients(m, c1, c2))
+predicate Invariant(m: DafnyState)
 {
-    // somehow need to prove that safety property
+    forall c1: Client, c2:Client, s: Server :: (RelationClientExists(m, c1) && RelationClientExists(m, c2) && RelationServerExists(m, s)) ==> (RelationLink(m, c1, s) && RelationLink(m, c2, s) ==> !RelationDifferentClients(m, c1, c2))
 }
-
-
